Update cpp2v-core to use val_related in tptsto_agree; models are not fully updated

theories/lang/cpp/logic/layout.v
@@ -13,6 +13,7 @@ From bedrock.lang.cpp.logic Require Import
 Require Import bedrock.lang.cpp.semantics.
 Require Import bedrock.lang.cpp.logic.z_to_bytes.
 Require Import bedrock.lang.cpp.logic.arr.
+Require Import bedrock.lang.cpp.logic.raw.
 
 Require Import bedrock.lang.cpp.heap_notations.
 
@@ -49,119 +50,6 @@ Section with_Σ.
   #[global] Existing Instance union_padding_strict_valid_observe.
   #[global] Instance union_padding_valid_observe q cls i : Observe validR (union_padding resolve q cls i).
   Proof. rewrite -svalidR_validR. apply _. Qed.
-
-  (** [raw_values_of_val σ ty v rs] states that the value [v] of type
-  [ty] is represented by the raw bytes in [rs]. WHat this means
-  depends on the type [ty]. *)
-  Axiom raw_bytes_of_val : genv -> type -> val -> list raw_byte -> Prop.
-
-  (** [raw_bytes_of_struct σ cls rss rs] states that the struct
-  consisting of fields of the raw bytes [rss] is represented by the
-  raw bytes in [rs]. [rs] should agree with [rss] on the offsets of
-  the fields. It might be possible to make some assumptions about the
-  parts of [rs] that represent padding based on the ABI. *)
-  Axiom raw_bytes_of_struct : genv -> globname -> gmap ident (list raw_byte) -> list raw_byte -> Prop.
-
-  Axiom raw_bytes_of_sizeof : forall ty v rs,
-     raw_bytes_of_val resolve ty v rs -> size_of resolve ty = Some (N.of_nat $ length rs).
-
-  (** [rawR q rs]: the argument pointer points to [raw_byte] [r] within the C++ abstract machine. *)
-  Definition rawR_def (q : Qp) (r : raw_byte) : Rep :=
-    as_Rep (fun p => tptsto T_uchar q p (Vraw r)).
-  Definition rawR_aux : seal (@rawR_def). Proof. by eexists. Qed.
-  Definition rawR := rawR_aux.(unseal).
-  Definition rawR_eq : @rawR = _ := rawR_aux.(seal_eq).
-  #[global] Arguments rawR q raw : rename.
-
-  #[global] Instance rawR_proper :
-    Proper ((=) ==> (=) ==> (⊣⊢)) (@rawR).
-  Proof. by intros ??-> ??->. Qed.
-  #[global] Instance rawR_mono :
-    Proper ((=) ==> (=) ==> (⊢)) (@rawR).
-  Proof. by intros ??-> ??->. Qed.
-
-  #[global] Instance rawR_affine q raw
-    : Affine (rawR q raw).
-  Proof. rewrite rawR_eq. apply _. Qed.
-  #[global] Instance rawR_timeless q raw
-    : Timeless (rawR q raw).
-  Proof. rewrite rawR_eq. apply _. Qed.
-
-  #[global] Instance rawR_fractional raw :
-    Fractional (λ q, rawR q raw).
-  Proof. rewrite rawR_eq. apply _. Qed.
-  #[global] Instance rawR_as_fractional q raw :
-    AsFractional (rawR q raw) (λ q, rawR q raw) q.
-  Proof. constructor. done. apply _. Qed.
-
-  #[global] Instance rawR_observe_frac_valid (q : Qp) raw :
-    Observe [| q ≤ 1 |]%Qp (rawR q raw).
-  Proof. rewrite rawR_eq. apply _. Qed.
-
-  #[global] Instance rawR_observe_agree q1 q2 raw1 raw2 :
-    Observe2 [| raw1 = raw2 |] (rawR q1 raw1) (rawR q2 raw2).
-  Proof.
-    rewrite rawR_eq/rawR_def.
-    apply: as_Rep_only_provable_observe_2=> p.
-    iIntros "Hptsto1 Hptsto2".
-    iPoseProof (tptsto_agree_raw with "Hptsto1 Hptsto2") as "%Hraws"; eauto.
-    iModIntro; iPureIntro; by inversion Hraws.
-  Qed.
-
-  Definition rawsR (q : Qp) (rs : list raw_byte) : Rep := arrayR T_uchar (rawR q) rs.
-
-  #[global] Instance rawsR_proper :
-    Proper ((=) ==> (=) ==> (⊣⊢)) (@rawsR).
-  Proof. by intros ??-> ??->. Qed.
-  #[global] Instance rawsR_mono :
-    Proper ((=) ==> (=) ==> (⊢)) (@rawsR).
-  Proof. by intros ??-> ??->. Qed.
-
-  #[global] Instance rawsR_affine q rs
-    : Affine (rawsR q rs).
-  Proof. apply _. Qed.
-  #[global] Instance rawsR_timeless q rs
-    : Timeless (rawsR q rs).
-  Proof. apply _. Qed.
-
-  #[global] Instance rawsR_fractional rs :
-    Fractional (λ q, rawsR q rs).
-  Proof. apply _. Qed.
-  #[global] Instance rawsR_as_fractional q rs :
-    AsFractional (rawsR q rs) (λ q, rawsR q rs) q.
-  Proof. constructor. done. apply _. Qed.
-
-  #[global] Instance rawsR_observe_frac_valid (q : Qp) rs :
-    (0 < length rs) ->
-    Observe [| q ≤ 1 |]%Qp (rawsR q rs).
-  Proof.
-    intros Hlen; rewrite /rawsR; induction rs;
-      by [ simpl in Hlen; lia
-         | rewrite arrayR_cons; apply _].
-  Qed.
-
-  #[global] Instance rawsR_observe_agree q1 q2 rs1 rs2 :
-    length rs1 = length rs2 ->
-    Observe2 [| rs1 = rs2 |] (rawsR q1 rs1) (rawsR q2 rs2).
-  Proof.
-    generalize dependent rs2; induction rs1 as [| r1 ? ?]; intros * Hlen.
-    - destruct rs2; [| simpl in Hlen; lia].
-      rewrite /Observe2; iIntros "? ? !>"; by iPureIntro.
-    - destruct rs2 as [| r2 ?]; [simpl in Hlen; lia |].
-      rewrite !cons_length in Hlen; inversion Hlen.
-      rewrite /rawsR !arrayR_cons;
-        fold (rawsR q1 rs1);
-        fold (rawsR q2 rs2).
-      iIntros "(Htype_ptrR1 & HrawR1 & HrawsR1)
-               (Htype_ptrR2 & HrawR2 & HrawsR2)".
-      iDestruct (observe_2 [| r1 = r2 |] with "HrawR1 HrawR2") as %->.
-      specialize (IHrs1 rs2 ltac:(auto)).
-      iDestruct (observe_2 [| rs1 = rs2 |] with "HrawsR1 HrawsR2") as %->.
-      iModIntro; by iPureIntro.
-  Qed.
-
-  Axiom primR_to_rawsR: forall ty q v,
-    primR ty q v -|- Exists rs, rawsR q rs ** [| raw_bytes_of_val resolve ty v rs |] ** type_ptrR ty.
 
   (* TODO: Do we need type_ptrR here? *)
   Axiom struct_to_raw : forall cls st rss q,
@@ -212,53 +100,4 @@ Section with_Σ.
     -|- _offsetR (_sub t (Z.of_N n)) validR **
         [∗list] i ↦ _ ∈ repeat () (BinNatDef.N.to_nat n),
                 _offsetR (_sub t (Z.of_nat i)) (anyR t 1).
-
-  Definition decodes (endianness: endian) (sgn: signed) (l: list N) (z: Z) :=
-    _Z_from_bytes endianness sgn l = z.
-
-  (* JH: TODO: Deprecate the following stuff *)
-  Definition decodes_uint (l : list N) (z : Z) :=
-    Unfold decodes (decodes (genv_byte_order resolve) Unsigned l z).
-
-  (* JH: TODO: Determine what new axioms we should add here. *)
-  Axiom raw_byte_of_int_eq : forall sz x rs,
-      raw_bytes_of_val resolve (Tint sz Unsigned) (Vint x) rs <-> (exists l, decodes_uint l x /\ rs = raw_int_byte <$> l).
-
-  Axiom raw_int_byte_primR : forall q r,
-      rawR q (raw_int_byte r) -|- primR T_uchar q (Vint (Z.of_N r)).
-
-  (** TODO: determine whether this is correct with respect to pointers *)
-  Lemma decode_uint_primR : forall q sz (x : Z),
-    primR (Tint sz Unsigned) q (Vint x) -|-
-    Exists l : list N,
-      arrayR (Tint W8 Unsigned) (fun c => primR (Tint W8 Unsigned) q (Vint c)) (Z.of_N <$> l) **
-      type_ptrR (Tint sz Unsigned) **
-      [| decodes_uint l x |].
-  Proof.
-    move => q sz x.
-    rewrite primR_to_rawsR. setoid_rewrite raw_byte_of_int_eq.
-    iSplit.
-    - iDestruct 1 as (rs) "(Hraw & H & $)".
-      iDestruct "H" as %[l [Hdec ->]].
-      iExists _; iSplit => //. clear Hdec.
-      rewrite /rawsR arrayR_eq/arrayR_def. iStopProof.
-      (* TODO i need to do induction here because the [Proper] instances are too weak. *)
-      induction l => // /=.
-      rewrite !arrR_cons; eauto.
-      rewrite -IHl /=. f_equiv. f_equiv.
-        by rewrite raw_int_byte_primR.
-    - iDestruct 1 as (l) "(Harray & $ & H)".
-      iDestruct "H" as %Hdec.
-      iExists _; iSplit => //; eauto with iFrame. clear Hdec.
-      rewrite /rawsR arrayR_eq/arrayR_def; iStopProof.
-      induction l => // /=.
-      rewrite !arrR_cons; eauto.
-      rewrite -IHl /=. f_equiv. f_equiv.
-        by rewrite raw_int_byte_primR.
-  Qed.
-
-  Axiom decode_uint_anyR : forall q sz,
-    anyR (Tint sz Unsigned) q -|-
-         anyR (Tarray T_uchar (bytesN sz)) q **
-         type_ptrR (Tint sz Unsigned).
 End with_Σ.
